\documentclass[11pt]{article}

\usepackage[a4paper, total={7in, 10.5in}]{geometry}
\usepackage{graphicx} % Required for inserting images
\usepackage{amsfonts}
\usepackage{amssymb}
\usepackage{amsmath}
\usepackage[T1]{fontenc}

\title{List 2 Exercise 1 PDF for UMSI}
\author{Mateusz Pe≈Çechaty}
\date{June 2024}

\begin{document}

\maketitle 

\section{Task Description}
Let $X \in \{0, 1\}$ 
be an input drawn from a Bernoulli distribution $B(p)$ $p < \frac{1}{2}$, 
and let $Y \in \{0, 1\}$ be the output obtained as follows:
$$
Y =
\begin{cases} 
X & \textrm{with probability } 1 - p, \\ 
1 - X & \textrm{with probability } p 
\end{cases}
$$
Determine the optimal Bayes classifier and its risk.

\section{Solution}

\subsubsection*{Bayes Classifier}
$h(y)$ chooses $x$ that maximizes possibility of hitting right value.

$$h(y) = \arg \max_{x \in {0, 1}} P(X=x | Y=y)$$

It means that 
$$h(0) = 0 \iff P(X=0 | Y=0) > P(X=1 | Y=0)$$
$$h(1) = 0 \iff P(X=0 | Y=1) > P(X=1 | Y=1)$$

So we need to calculate these probabilities and a lot of others.

\begin{itemize}
    \item From Task Description \\
    $P(X=0) = 1-p$ \\
    $P(X=1) = p$ \\
    $P(Y=0 | X = 0) = 1-p$ \\
    $P(Y=0 | X=1) = p$ \\
    $P(Y=1 | X=0) = p$ \\
    $P(Y=1 | X=1) = 1-p$ 
    \item Marginal Probabilities \\
    $P(Y=0) = P(Y=0 \land X=0) + P(Y=0 \land X=1) = (1-p)^2 + p^2$ \\
    $P(Y=1) = P(Y=1 \land X=0) + P(Y=1 \land X=1) = (1-p)\cdot p + (1-p)\cdot p$ 
    \item Posterior Probabilities from Bayes \\
    $P(X=0 | Y=0) = \frac{(1-p)^2}{(1-p)^2 + p^2}$ \\
    $P(X=1 | Y=0) = \frac{p^2}{(1-p)^2 + p^2}$ \\
    $P(X=0 | Y=1) = \frac{p\cdot(1-p)}{2p\cdot(1-p)}$ \\
    $P(X=1 | Y=1) = \frac{p \cdot(1-p)}{2p\cdot(1-p)}$ 
\end{itemize}
From above we can say that $h(0) = 0$, because for $p < \frac{1}{2}$, we have $p^2 < (1-p)^2$. \\
On the other hand, as $P(X=0|Y=1) = P(X=1|Y=1)$, we can choose any value for $h(1)$ so for symmetry we choose $h(1) = 1$

\subsubsection*{Risk}
$$L^* = P(X=0) \min{P(Y=1 | X=0), P(Y=0|X=0)} + P(X=1)\min{P(Y=1|X=1), P(Y=0|X=1)}$$
$$L^* = (1-p)\cdot(p) + p^2 = p$$

\end{document}
